libcrux-iot/sha3/proofs/lean/LibcruxIotSha3/Extraction/Funs.lean
@@ -4481,34 +4481,34 @@ def lane.Lane2U32.Insts.CoreConvertFromArrayU322 : core.convert.From
 }
 
 /-- [libcrux_iot_sha3::SHA3_224_DIGEST_SIZE]
-    Source: 'sha3/src/lib.rs', lines 75:0-75:43
+    Source: 'sha3/src/lib.rs', lines 77:0-77:43
     Visibility: public -/
 @[global_simps, irreducible] def SHA3_224_DIGEST_SIZE : Std.Usize := 28#usize
 
 /-- [libcrux_iot_sha3::SHA3_256_DIGEST_SIZE]
-    Source: 'sha3/src/lib.rs', lines 77:0-77:43
+    Source: 'sha3/src/lib.rs', lines 79:0-79:43
     Visibility: public -/
 @[global_simps, irreducible] def SHA3_256_DIGEST_SIZE : Std.Usize := 32#usize
 
 /-- [libcrux_iot_sha3::SHA3_384_DIGEST_SIZE]
-    Source: 'sha3/src/lib.rs', lines 79:0-79:43
+    Source: 'sha3/src/lib.rs', lines 81:0-81:43
     Visibility: public -/
 @[global_simps, irreducible] def SHA3_384_DIGEST_SIZE : Std.Usize := 48#usize
 
 /-- [libcrux_iot_sha3::SHA3_512_DIGEST_SIZE]
-    Source: 'sha3/src/lib.rs', lines 81:0-81:43
+    Source: 'sha3/src/lib.rs', lines 83:0-83:43
     Visibility: public -/
 @[global_simps, irreducible] def SHA3_512_DIGEST_SIZE : Std.Usize := 64#usize
 
 /-- [libcrux_iot_sha3::{impl core::clone::Clone for libcrux_iot_sha3::Algorithm}::clone]:
-    Source: 'sha3/src/lib.rs', lines 89:39-89:44
+    Source: 'sha3/src/lib.rs', lines 91:39-91:44
     Visibility: public -/
 def Algorithm.Insts.CoreCloneClone.clone
   (self : Algorithm) : RustM Algorithm := do
   ok self
 
 /-- Trait implementation: [libcrux_iot_sha3::{impl core::clone::Clone for libcrux_iot_sha3::Algorithm}]
-    Source: 'sha3/src/lib.rs', lines 89:39-89:44 -/
+    Source: 'sha3/src/lib.rs', lines 91:39-91:44 -/
 @[reducible]
 impl_def Algorithm.Insts.CoreCloneClone : core.clone.Clone Algorithm := {
   clone := Algorithm.Insts.CoreCloneClone.clone
@@ -4517,21 +4517,21 @@ impl_def Algorithm.Insts.CoreCloneClone : core.clone.Clone Algorithm := {
 }
 
 /-- Trait implementation: [libcrux_iot_sha3::{impl core::marker::Copy for libcrux_iot_sha3::Algorithm}]
-    Source: 'sha3/src/lib.rs', lines 89:33-89:37 -/
+    Source: 'sha3/src/lib.rs', lines 91:33-91:37 -/
 @[reducible]
 def Algorithm.Insts.CoreMarkerCopy : core.marker.Copy Algorithm := {
   cloneCloneInst := Algorithm.Insts.CoreCloneClone
 }
 
 /-- Trait implementation: [libcrux_iot_sha3::{impl core::marker::StructuralPartialEq for libcrux_iot_sha3::Algorithm}]
-    Source: 'sha3/src/lib.rs', lines 89:46-89:55 -/
+    Source: 'sha3/src/lib.rs', lines 91:46-91:55 -/
 @[reducible]
 def Algorithm.Insts.CoreMarkerStructuralPartialEq :
   core.marker.StructuralPartialEq Algorithm := {
 }
 
 /-- [libcrux_iot_sha3::{impl core::cmp::PartialEq<libcrux_iot_sha3::Algorithm> for libcrux_iot_sha3::Algorithm}::eq]:
-    Source: 'sha3/src/lib.rs', lines 89:46-89:55
+    Source: 'sha3/src/lib.rs', lines 91:46-91:55
     Visibility: public -/
 def Algorithm.Insts.CoreCmpPartialEqAlgorithm.eq
   (self : Algorithm) (other : Algorithm) : RustM Bool := do
@@ -4540,7 +4540,7 @@ def Algorithm.Insts.CoreCmpPartialEqAlgorithm.eq
   ok (self1 = other1)
 
 /-- Trait implementation: [libcrux_iot_sha3::{impl core::cmp::PartialEq<libcrux_iot_sha3::Algorithm> for libcrux_iot_sha3::Algorithm}]
-    Source: 'sha3/src/lib.rs', lines 89:46-89:55 -/
+    Source: 'sha3/src/lib.rs', lines 91:46-91:55 -/
 @[reducible]
 impl_def Algorithm.Insts.CoreCmpPartialEqAlgorithm : core.cmp.PartialEq
   Algorithm Algorithm := {
@@ -4549,7 +4549,7 @@ impl_def Algorithm.Insts.CoreCmpPartialEqAlgorithm : core.cmp.PartialEq
 }
 
 /-- [libcrux_iot_sha3::{impl core::convert::From<u32> for libcrux_iot_sha3::Algorithm}::from]:
-    Source: 'sha3/src/lib.rs', lines 108:4-116:5
+    Source: 'sha3/src/lib.rs', lines 110:4-118:5
     Visibility: public -/
 def Algorithm.Insts.CoreConvertFromU32.from
   (v : Std.U32) : RustM Algorithm := do
@@ -4561,7 +4561,7 @@ def Algorithm.Insts.CoreConvertFromU32.from
   | _ => fail panic
 
 /-- Trait implementation: [libcrux_iot_sha3::{impl core::convert::From<u32> for libcrux_iot_sha3::Algorithm}]
-    Source: 'sha3/src/lib.rs', lines 107:0-117:1 -/
+    Source: 'sha3/src/lib.rs', lines 109:0-119:1 -/
 @[reducible]
 def Algorithm.Insts.CoreConvertFromU32 : core.convert.From Algorithm Std.U32
   := {
@@ -4569,7 +4569,7 @@ def Algorithm.Insts.CoreConvertFromU32 : core.convert.From Algorithm Std.U32
 }
 
 /-- [libcrux_iot_sha3::{impl core::convert::From<libcrux_iot_sha3::Algorithm> for u32}::from]:
-    Source: 'sha3/src/lib.rs', lines 120:4-127:5
+    Source: 'sha3/src/lib.rs', lines 122:4-129:5
     Visibility: public -/
 def U32.Insts.CoreConvertFromAlgorithm.from
   (v : Algorithm) : RustM Std.U32 := do
@@ -4580,7 +4580,7 @@ def U32.Insts.CoreConvertFromAlgorithm.from
   | Algorithm.Sha512 => ok 4#u32
 
 /-- Trait implementation: [libcrux_iot_sha3::{impl core::convert::From<libcrux_iot_sha3::Algorithm> for u32}]
-    Source: 'sha3/src/lib.rs', lines 119:0-128:1 -/
+    Source: 'sha3/src/lib.rs', lines 121:0-130:1 -/
 @[reducible]
 def U32.Insts.CoreConvertFromAlgorithm : core.convert.From Std.U32 Algorithm
   := {
@@ -4588,7 +4588,7 @@ def U32.Insts.CoreConvertFromAlgorithm : core.convert.From Std.U32 Algorithm
 }
 
 /-- [libcrux_iot_sha3::digest_size]:
-    Source: 'sha3/src/lib.rs', lines 131:0-138:1
+    Source: 'sha3/src/lib.rs', lines 133:0-140:1
     Visibility: public -/
 def digest_size (mode : Algorithm) : RustM Std.Usize := do
   match mode with
@@ -4598,7 +4598,7 @@ def digest_size (mode : Algorithm) : RustM Std.Usize := do
   | Algorithm.Sha512 => ok SHA3_512_DIGEST_SIZE
 
 /-- [libcrux_iot_sha3::keccakx1]:
-    Source: 'sha3/src/lib.rs', lines 620:0-622:1 -/
+    Source: 'sha3/src/lib.rs', lines 616:0-618:1 -/
 def keccakx1
   (RATE : Std.Usize) (DELIM : Std.U8) (data : Slice Std.U8)
   (out : Slice Std.U8) :
@@ -4607,7 +4607,7 @@ def keccakx1
   keccak.keccak RATE DELIM data out
 
 /-- [libcrux_iot_sha3::sha512_ema]:
-    Source: 'sha3/src/lib.rs', lines 333:0-340:1
+    Source: 'sha3/src/lib.rs', lines 335:0-342:1
     Visibility: public -/
 def sha512_ema
   (digest : Slice Std.U8) (payload : Slice Std.U8) : RustM (Slice Std.U8) := do
@@ -4619,7 +4619,7 @@ def sha512_ema
   keccakx1 72#usize 6#u8 payload digest
 
 /-- [libcrux_iot_sha3::sha384_ema]:
-    Source: 'sha3/src/lib.rs', lines 291:0-298:1
+    Source: 'sha3/src/lib.rs', lines 293:0-300:1
     Visibility: public -/
 def sha384_ema
   (digest : Slice Std.U8) (payload : Slice Std.U8) : RustM (Slice Std.U8) := do
@@ -4631,7 +4631,7 @@ def sha384_ema
   keccakx1 104#usize 6#u8 payload digest
 
 /-- [libcrux_iot_sha3::sha256_ema]:
-    Source: 'sha3/src/lib.rs', lines 249:0-256:1
+    Source: 'sha3/src/lib.rs', lines 251:0-258:1
     Visibility: public -/
 def sha256_ema
   (digest : Slice Std.U8) (payload : Slice Std.U8) : RustM (Slice Std.U8) := do
@@ -4643,7 +4643,7 @@ def sha256_ema
   keccakx1 136#usize 6#u8 payload digest
 
 /-- [libcrux_iot_sha3::sha224_ema]:
-    Source: 'sha3/src/lib.rs', lines 212:0-219:1
+    Source: 'sha3/src/lib.rs', lines 214:0-221:1
     Visibility: public -/
 def sha224_ema
   (digest : Slice Std.U8) (payload : Slice Std.U8) : RustM (Slice Std.U8) := do
@@ -4655,7 +4655,7 @@ def sha224_ema
   keccakx1 144#usize 6#u8 payload digest
 
 /-- [libcrux_iot_sha3::hash]:
-    Source: 'sha3/src/lib.rs', lines 151:0-175:1
+    Source: 'sha3/src/lib.rs', lines 153:0-177:1
     Visibility: public -/
 def hash
   (LEN : Std.Usize) (algorithm : Algorithm) (payload : Slice Std.U8) :
@@ -4701,7 +4701,7 @@ def hash
     ok (index_mut_back s1)
 
 /-- [libcrux_iot_sha3::sha224]:
-    Source: 'sha3/src/lib.rs', lines 184:0-195:1
+    Source: 'sha3/src/lib.rs', lines 186:0-197:1
     Visibility: public -/
 def sha224 (payload : Slice Std.U8) : RustM (Array Std.U8 28#usize) := do
   let a := Array.repeat 28#usize 0#u8
@@ -4715,7 +4715,7 @@ def sha224 (payload : Slice Std.U8) : RustM (Array Std.U8 28#usize) := do
   ok (index_mut_back s1)
 
 /-- [libcrux_iot_sha3::sha256]:
-    Source: 'sha3/src/lib.rs', lines 226:0-237:1
+    Source: 'sha3/src/lib.rs', lines 228:0-239:1
     Visibility: public -/
 def sha256 (payload : Slice Std.U8) : RustM (Array Std.U8 32#usize) := do
   let a := Array.repeat 32#usize 0#u8
@@ -4729,7 +4729,7 @@ def sha256 (payload : Slice Std.U8) : RustM (Array Std.U8 32#usize) := do
   ok (index_mut_back s1)
 
 /-- [libcrux_iot_sha3::sha384]:
-    Source: 'sha3/src/lib.rs', lines 263:0-274:1
+    Source: 'sha3/src/lib.rs', lines 265:0-276:1
     Visibility: public -/
 def sha384 (payload : Slice Std.U8) : RustM (Array Std.U8 48#usize) := do
   let a := Array.repeat 48#usize 0#u8
@@ -4743,7 +4743,7 @@ def sha384 (payload : Slice Std.U8) : RustM (Array Std.U8 48#usize) := do
   ok (index_mut_back s1)
 
 /-- [libcrux_iot_sha3::sha512]:
-    Source: 'sha3/src/lib.rs', lines 305:0-316:1
+    Source: 'sha3/src/lib.rs', lines 307:0-318:1
     Visibility: public -/
 def sha512 (payload : Slice Std.U8) : RustM (Array Std.U8 64#usize) := do
   let a := Array.repeat 64#usize 0#u8
@@ -4757,7 +4757,7 @@ def sha512 (payload : Slice Std.U8) : RustM (Array Std.U8 64#usize) := do
   ok (index_mut_back s1)
 
 /-- [libcrux_iot_sha3::shake128]:
-    Source: 'sha3/src/lib.rs', lines 352:0-363:1
+    Source: 'sha3/src/lib.rs', lines 351:0-362:1
     Visibility: public -/
 def shake128
   (BYTES : Std.Usize) (data : Slice Std.U8) : RustM (Array Std.U8 BYTES) := do
@@ -4772,14 +4772,14 @@ def shake128
   ok (index_mut_back s1)
 
 /-- [libcrux_iot_sha3::shake128_ema]:
-    Source: 'sha3/src/lib.rs', lines 372:0-374:1
+    Source: 'sha3/src/lib.rs', lines 371:0-373:1
     Visibility: public -/
 def shake128_ema
   (out : Slice Std.U8) (data : Slice Std.U8) : RustM (Slice Std.U8) := do
   keccakx1 168#usize 31#u8 data out
 
 /-- [libcrux_iot_sha3::shake256]:
-    Source: 'sha3/src/lib.rs', lines 386:0-397:1
+    Source: 'sha3/src/lib.rs', lines 382:0-393:1
     Visibility: public -/
 def shake256
   (BYTES : Std.Usize) (data : Slice Std.U8) : RustM (Array Std.U8 BYTES) := do
@@ -4794,28 +4794,28 @@ def shake256
   ok (index_mut_back s1)
 
 /-- [libcrux_iot_sha3::shake256_ema]:
-    Source: 'sha3/src/lib.rs', lines 406:0-408:1
+    Source: 'sha3/src/lib.rs', lines 402:0-404:1
     Visibility: public -/
 def shake256_ema
   (out : Slice Std.U8) (data : Slice Std.U8) : RustM (Slice Std.U8) := do
   keccakx1 136#usize 31#u8 data out
 
 /-- Trait implementation: [libcrux_iot_sha3::incremental::private::{impl libcrux_iot_sha3::incremental::private::Sealed for libcrux_iot_sha3::incremental::Shake128Xof}]
-    Source: 'sha3/src/lib.rs', lines 433:8-433:45 -/
+    Source: 'sha3/src/lib.rs', lines 429:8-429:45 -/
 @[reducible]
 def incremental.Shake128Xof.Insts.Libcrux_iot_sha3IncrementalPrivateSealed :
   incremental.private.Sealed incremental.Shake128Xof := {
 }
 
 /-- Trait implementation: [libcrux_iot_sha3::incremental::private::{impl libcrux_iot_sha3::incremental::private::Sealed for libcrux_iot_sha3::incremental::Shake256Xof}]
-    Source: 'sha3/src/lib.rs', lines 434:8-434:45 -/
+    Source: 'sha3/src/lib.rs', lines 430:8-430:45 -/
 @[reducible]
 def incremental.Shake256Xof.Insts.Libcrux_iot_sha3IncrementalPrivateSealed :
   incremental.private.Sealed incremental.Shake256Xof := {
 }
 
 /-- [libcrux_iot_sha3::incremental::{impl libcrux_iot_sha3::incremental::Xof<168usize> for libcrux_iot_sha3::incremental::Shake128Xof}::squeeze]:
-    Source: 'sha3/src/lib.rs', lines 514:8-516:9
+    Source: 'sha3/src/lib.rs', lines 510:8-512:9
     Visibility: public -/
 def incremental.Shake128Xof.Insts.Libcrux_iot_sha3IncrementalXof168.squeeze
   (self : incremental.Shake128Xof) (out : Slice Std.U8) :
@@ -4825,7 +4825,7 @@ def incremental.Shake128Xof.Insts.Libcrux_iot_sha3IncrementalXof168.squeeze
   ok ({ state := kxs }, out1)
 
 /-- [libcrux_iot_sha3::incremental::{impl libcrux_iot_sha3::incremental::Xof<168usize> for libcrux_iot_sha3::incremental::Shake128Xof}::absorb_final]:
-    Source: 'sha3/src/lib.rs', lines 510:8-512:9
+    Source: 'sha3/src/lib.rs', lines 506:8-508:9
     Visibility: public -/
 def
   incremental.Shake128Xof.Insts.Libcrux_iot_sha3IncrementalXof168.absorb_final
@@ -4836,7 +4836,7 @@ def
   ok { state := kxs }
 
 /-- [libcrux_iot_sha3::incremental::{impl libcrux_iot_sha3::incremental::Xof<168usize> for libcrux_iot_sha3::incremental::Shake128Xof}::absorb]:
-    Source: 'sha3/src/lib.rs', lines 502:8-504:9
+    Source: 'sha3/src/lib.rs', lines 498:8-500:9
     Visibility: public -/
 def incremental.Shake128Xof.Insts.Libcrux_iot_sha3IncrementalXof168.absorb
   (self : incremental.Shake128Xof) (input : Slice Std.U8) :
@@ -4846,7 +4846,7 @@ def incremental.Shake128Xof.Insts.Libcrux_iot_sha3IncrementalXof168.absorb
   ok { state := kxs }
 
 /-- [libcrux_iot_sha3::incremental::{impl libcrux_iot_sha3::incremental::Xof<168usize> for libcrux_iot_sha3::incremental::Shake128Xof}::new]:
-    Source: 'sha3/src/lib.rs', lines 493:8-497:9
+    Source: 'sha3/src/lib.rs', lines 489:8-493:9
     Visibility: public -/
 def incremental.Shake128Xof.Insts.Libcrux_iot_sha3IncrementalXof168.new
   : RustM incremental.Shake128Xof := do
@@ -4854,7 +4854,7 @@ def incremental.Shake128Xof.Insts.Libcrux_iot_sha3IncrementalXof168.new
   ok { state := kxs }
 
 /-- Trait implementation: [libcrux_iot_sha3::incremental::{impl libcrux_iot_sha3::incremental::Xof<168usize> for libcrux_iot_sha3::incremental::Shake128Xof}]
-    Source: 'sha3/src/lib.rs', lines 492:4-517:5 -/
+    Source: 'sha3/src/lib.rs', lines 488:4-513:5 -/
 @[reducible]
 def incremental.Shake128Xof.Insts.Libcrux_iot_sha3IncrementalXof168 :
   incremental.Xof incremental.Shake128Xof 168#usize := {
@@ -4870,7 +4870,7 @@ def incremental.Shake128Xof.Insts.Libcrux_iot_sha3IncrementalXof168 :
 }
 
 /-- [libcrux_iot_sha3::incremental::{impl libcrux_iot_sha3::incremental::Xof<136usize> for libcrux_iot_sha3::incremental::Shake256Xof}::squeeze]:
-    Source: 'sha3/src/lib.rs', lines 544:8-546:9
+    Source: 'sha3/src/lib.rs', lines 540:8-542:9
     Visibility: public -/
 def incremental.Shake256Xof.Insts.Libcrux_iot_sha3IncrementalXof136.squeeze
   (self : incremental.Shake256Xof) (out : Slice Std.U8) :
@@ -4880,7 +4880,7 @@ def incremental.Shake256Xof.Insts.Libcrux_iot_sha3IncrementalXof136.squeeze
   ok ({ state := kxs }, out1)
 
 /-- [libcrux_iot_sha3::incremental::{impl libcrux_iot_sha3::incremental::Xof<136usize> for libcrux_iot_sha3::incremental::Shake256Xof}::absorb_final]:
-    Source: 'sha3/src/lib.rs', lines 539:8-541:9
+    Source: 'sha3/src/lib.rs', lines 535:8-537:9
     Visibility: public -/
 def
   incremental.Shake256Xof.Insts.Libcrux_iot_sha3IncrementalXof136.absorb_final
@@ -4891,7 +4891,7 @@ def
   ok { state := kxs }
 
 /-- [libcrux_iot_sha3::incremental::{impl libcrux_iot_sha3::incremental::Xof<136usize> for libcrux_iot_sha3::incremental::Shake256Xof}::absorb]:
-    Source: 'sha3/src/lib.rs', lines 531:8-533:9
+    Source: 'sha3/src/lib.rs', lines 527:8-529:9
     Visibility: public -/
 def incremental.Shake256Xof.Insts.Libcrux_iot_sha3IncrementalXof136.absorb
   (self : incremental.Shake256Xof) (input : Slice Std.U8) :
@@ -4901,7 +4901,7 @@ def incremental.Shake256Xof.Insts.Libcrux_iot_sha3IncrementalXof136.absorb
   ok { state := kxs }
 
 /-- [libcrux_iot_sha3::incremental::{impl libcrux_iot_sha3::incremental::Xof<136usize> for libcrux_iot_sha3::incremental::Shake256Xof}::new]:
-    Source: 'sha3/src/lib.rs', lines 521:8-525:9
+    Source: 'sha3/src/lib.rs', lines 517:8-521:9
     Visibility: public -/
 def incremental.Shake256Xof.Insts.Libcrux_iot_sha3IncrementalXof136.new
   : RustM incremental.Shake256Xof := do
@@ -4909,7 +4909,7 @@ def incremental.Shake256Xof.Insts.Libcrux_iot_sha3IncrementalXof136.new
   ok { state := kxs }
 
 /-- Trait implementation: [libcrux_iot_sha3::incremental::{impl libcrux_iot_sha3::incremental::Xof<136usize> for libcrux_iot_sha3::incremental::Shake256Xof}]
-    Source: 'sha3/src/lib.rs', lines 520:4-547:5 -/
+    Source: 'sha3/src/lib.rs', lines 516:4-543:5 -/
 @[reducible]
 def incremental.Shake256Xof.Insts.Libcrux_iot_sha3IncrementalXof136 :
   incremental.Xof incremental.Shake256Xof 136#usize := {
